trying to implement booleans

VerifiedCompiler/Ast.lean
@@ -1,4 +1,8 @@
 inductive Expr
+| Bool (b : Bool)
 | Num (n : Nat)
 | Add1 (e : Expr)
 | Sub1 (e : Expr)
+
+-- Add1 (Add1 (Sub1 (Add1 (Num 10)))) -> 12
+-- 0101, 01010101, 10101 -> 12
