VerifiedCompiler/Compare.lean
@@ -3,47 +3,78 @@ import VerifiedCompiler.Compile
 import VerifiedCompiler.Interpret
 
 import VerifiedCompiler.LoVelib
+import Mathlib.Data.Int.Bitwise
 
 open Value Expr
 
 def Processor.evalToValue (ds : List Directive) : Value :=
-  Integer (Processor.eval ds)
+  match Processor.eval ds with
+  | Sum.inl n => Integer n
+  | Sum.inr b => Boolean b
 
+theorem shl_shr (n sh : Nat) : n <<< sh >>> sh = n :=
+  by
+    sorry
 
-theorem correctness :
-  ∀ prog : Expr, Processor.evalToValue (compile_expr prog) = interpret_expr prog
+theorem smth (n sh : Nat) : (n * sh ^ 2) >>> sh = n := sorry
+
+theorem land_helper (n : Nat) : n * 2 ^ 2 &&& 3 = 0 := sorry
+
+-- the compiler will produce the same value when the interpreter produces a some
+-- change the correctness theorem to say that the interpreter produces a some
+
+thoerem compile_smth : ∀ b : Bool, compile_expr (Expr.Bool b) =
+
+theorem correctness : ∀ prog : Expr,
+  (interpret_expr prog).isSome →
+  Processor.evalToValue (compile_expr prog) = interpret_expr prog
   | Expr.Num n =>
     by
-      simp [Processor.evalToValue, Processor.eval, Processor.evalToState,
-      processDirective, ProcessorState.setReg, ProcessorState.opVal, interpret_expr]
+      simp [Processor.evalToValue, Processor.eval, Processor.evalToState, processDirective, compile_expr, interpret_expr, List.foldl, ProcessorState.setReg, ProcessorState.opVal]
+      simp [num_tag, num_shift, num_mask, land_helper, shl_shr, smth]
+
+  | Expr.Bool b =>
+    by
+      simp [Processor.evalToValue, Processor.eval, Processor.evalToState, compile_expr]
+      simp [bool_tag, bool_shift, bool_mask]
+
 
   | Expr.Sub1 e =>
     by
-      have ih := correctness e
-      simp [Processor.evalToValue, Processor.eval, Processor.evalToState, interpret_expr] at *
-      rw [←ih]
-      simp
-      rw [compile_expr]
-      cases (compile_expr e) with
-      | nil => simp
-      | cons hd tl =>
-        have hfold_concat :=
-          List.foldl_concat processDirective { rax := 0 }
-            (Directive.Sub (Operand.Reg Register.Rax, Operand.Imm 1)) (hd :: tl)
-        rw [hfold_concat]
-        rfl
+      -- have ih := correctness e
+      -- simp [Processor.evalToValue, Processor.eval, Processor.evalToState, interpret_expr] at *
+      -- rw [←ih]
+      -- simp
+      -- rw [compile_expr]
+      -- sorry
+      -- cases (compile_expr e) with
+      -- | nil =>
+      --   simp
+      --   sorry
+
+      -- | cons hd tl =>
+      --   have hfold_concat :=
+      --     List.foldl_concat processDirective { rax := 0 }
+      --       (Directive.Sub (Operand.Reg Register.Rax, Operand.Imm 1)) (hd :: tl)
+      --   -- rw [hfold_concat]
+        -- rfl
+        sorry
 
   | Expr.Add1 e =>
     by
-      have ih := correctness e
-      simp [Processor.evalToValue, Processor.eval, Processor.evalToState, interpret_expr] at *
-      rw [←ih]
-      simp
-      rw [compile_expr]
-      cases (compile_expr e) with
-      | nil => simp
-      | cons hd tl =>
-        have hfold_concat := List.foldl_concat processDirective { rax := 0 }
-            (Directive.Add (Operand.Reg Register.Rax, Operand.Imm 1)) (hd :: tl)
-        rw [hfold_concat]
-        rfl
+      -- have ih := correctness e
+      -- simp [Processor.evalToValue, Processor.eval, Processor.evalToState, interpret_expr] at *
+      -- rw [←ih]
+      -- simp
+      -- rw [compile_expr]
+      -- sorry
+      -- cases (compile_expr e) with
+      -- | nil =>
+      --   simp
+      --   sorry
+      -- | cons hd tl =>
+      --   have hfold_concat := List.foldl_concat processDirective { rax := 0 }
+      --       (Directive.Add (Operand.Reg Register.Rax, Operand.Imm 1)) (hd :: tl)
+        -- rw [hfold_concat]
+        -- rfl
+        sorry
