VerifiedCompiler/Compile.lean
@@ -3,10 +3,22 @@ import VerifiedCompiler.Ast
 
 open Directive Operand Register Expr
 
+def num_shift := 2
+def num_mask := 0b11
+def num_tag := 0b00
+
+def bool_shift := 7
+def bool_mask := 0b1111111
+def bool_tag := 0b0011111
+
 def compile_expr : Expr → List Directive
 | Num n =>
-  [Mov (Reg Rax, Imm n)]
+  [Mov (Reg Rax, Imm (n <<< num_shift))]
+| Expr.Bool b =>
+  match b with
+  | true => [Mov (Reg Rax, Imm ((1 <<< bool_shift) ||| bool_tag))]
+  | false => [Mov (Reg Rax, Imm ((0 <<< bool_shift) ||| bool_tag))]
 | Sub1 e =>
-  (compile_expr e) ++ [Sub (Reg Rax, Imm 1)]
+  (compile_expr e) ++ [Sub (Reg Rax, Imm (1 <<< num_shift))]
 | Add1 e =>
-  (compile_expr e) ++ [Add (Reg Rax, Imm 1)]
+  (compile_expr e) ++ [Add (Reg Rax, Imm (1 <<< num_shift))]
