VerifiedCompiler/Interpret.lean
@@ -5,14 +5,18 @@ open Directive Operand Register Expr
 
 inductive Value
 | Integer (i : Nat)
+| Boolean (b : Bool)
 
 open Value
 
-def interpret_expr : Expr → Value
-| Num n => Integer n
+def interpret_expr : Expr → Option Value
+| Num n => some (Integer n)
+| Expr.Bool b => some (Boolean b)
 | Add1 e =>
   match (interpret_expr e) with
-  | Integer i => Integer (i + 1)
+  | Integer i => some (Integer (i + 1))
+  | _ => none
 | Sub1 e =>
   match (interpret_expr e) with
-  | Integer i => Integer (i - 1)
+  | Integer i => some (Integer (i - 1))
+  | _ => none
